

1. Solve the DEs

(1) $xy' = y^2 + y$

$\hookrightarrow \frac{1}{y^2+y} dy = \frac{1}{x} dx$

$\frac{1}{y(y+1)} dy = \left(\frac{1}{y} - \frac{1}{y+1} \right) dy = \frac{1}{x} dx$

$\int \left(\frac{1}{y} - \frac{1}{y+1} \right) dy = \int \frac{1}{x} dx$

$\ln|y| - \ln|y+1| = \ln|x| + C$

$\ln \left| \frac{y}{y+1} \right| = \ln|x| + C$

$\frac{y}{y+1} = C \cdot x$

$1 + \frac{1}{y+1} = C \cdot x$

$\frac{1}{y+1} = 1 - C \cdot x$

$y+1 = \frac{1}{1-C \cdot x}$

$y = \frac{1}{1-C \cdot x} - 1 = \frac{C \cdot x}{1-C \cdot x} = \frac{x}{\frac{1}{C} - x} = \frac{x}{C-x}$

$\therefore \boxed{y = \frac{x}{C-x}}$

(3) $x \frac{dy}{dx} + y = x^2 y^2$

$\hookrightarrow y' + \frac{1}{x} y = x y^2$

$u = y^{-1} = y^{-1}$

$u' = -y^{-2} \cdot y'$

$y' = -\frac{u'}{u^2}$

$\therefore -\frac{u'}{u^2} + \frac{1}{x} \cdot \frac{1}{u} = x \frac{1}{u^2}$

$u' - \frac{u}{x} = -x$

(2) $\frac{dy}{dx} = y^2 - 4$

$\hookrightarrow \frac{1}{y^2-4} dy = dx$

$\frac{1}{(y+2)(y-2)} dy = dx$

$\frac{1}{4} \left(\frac{1}{y-2} - \frac{1}{y+2} \right) dy = \int dx$

$\frac{1}{4} \left[\ln|y-2| - \ln|y+2| \right] = x + C$

$\ln \left| \frac{y-2}{y+2} \right| = 4x + C$

$\frac{y-2}{y+2} = C \cdot e^{4x}$

$1 + \frac{-4}{y+2} = C \cdot e^{4x}$

$\frac{4}{y+2} = 1 - C \cdot e^{4x}$

$y = \frac{4}{1 - C \cdot e^{4x}} - 2$

$\boxed{y = \frac{2 + 2 \cdot C \cdot e^{4x}}{1 - C \cdot e^{4x}}}$

$(x - \frac{u}{x}) dx + \frac{1}{x} du = 0$

$\frac{P(x,y)}{Q(x,y)}$

$P_y = -\frac{1}{x} \quad Q_x = 0$

$\frac{1}{x} (P_y - Q_x) = A(x) = -\frac{1}{x}$

$\therefore F(x) = e^{\int -\frac{1}{x} dx} = e^{-\ln|x|} = e^{\ln|\frac{1}{x}|} = \frac{1}{x}$

$\frac{1}{x} u' - \frac{u}{x^2} = -1$

$(1 - \frac{u}{x}) dx + \frac{1}{x} du = 0$

$M_u = -\frac{1}{x^2} = N_x = -\frac{1}{x^2}$

$u(x,y) = \frac{1}{x} u + g(x) = 0$

$u_x(x,y) = -\frac{1}{x^2} u + g'(x) = -\frac{u}{x^2} + 1$

$\therefore g'(x) = 1$

$g(x) = x + C$

$u(x,y) = \frac{1}{x} u + x + C = \frac{1}{x} \frac{1}{y} + x + C$

$\therefore \boxed{y = \frac{1}{Cx - x^2}}$

$$(4) \frac{dy}{dx} = (-2x+y)^2 - 1, y(0) = 0$$

$$u(x) = -2x + y$$

$$u' = -2 + y'$$

$$y' = u' + 2 = u^2 - 1$$

$$u' = u^2 - 1$$

$$dx = \frac{1}{u^2 - 1} du = \frac{1}{(u-1)(u+1)} du = \frac{1}{2} \left(\frac{1}{u-1} - \frac{1}{u+1} \right) du$$

$$\int \frac{1}{2} \left(\frac{1}{u-1} - \frac{1}{u+1} \right) du = \int 1 \cdot dx$$

$$\frac{1}{2} (\ln|u-1| - \ln|u+1|) = x + C$$

$$\ln \left| \frac{u-1}{u+1} \right| = 2x + C$$

$$\frac{u-1}{u+1} = C e^{2x}$$

$$1 + \frac{-6}{u+1} = C e^{6x}$$

$$\frac{-6}{u+1} = C e^{6x} - 1$$

$$\frac{u+1}{-6} = \frac{C e^{6x} - 1}{1 - C e^{6x}}$$

$$u = \frac{1 - C e^{6x}}{1 - C e^{6x}} - 3 = \frac{3 + 3C e^{6x}}{1 - C e^{6x}}$$

$$-2x + y$$

$$y = 2x + \frac{3(1 + C e^{6x})}{1 - C e^{6x}}$$

$$y(0) = 0, 0 = 0 + \frac{3(1+C)}{1-C}, \therefore C = -1$$

$$\boxed{y = 2x + \frac{3(1 - e^{6x})}{1 + e^{6x}}}$$

$$(5) \frac{dy}{dx} + y = 2x, y(0) = 4$$

$$y' + y = 2x$$

$$(y-x)dx + 1 \cdot dy = 0$$

$$\underbrace{p}_P \underbrace{Q}_Q$$

$$p_y = 1, Q_x = 0$$

$$\frac{1}{Q} (p_y - Q_x) = 1 = R(x)$$

$$F(x) = \int 1 dx = e^x$$

$$\frac{e^x (y-x) dx}{M} + \frac{e^x dy}{N} = 0$$

$$M_y = e^x = N_x = e^x$$

$$u(x, y) = \int e^x dy = e^x y + g(x)$$

$$u_x = e^x y + g'(x) = e^x y - x e^x$$

$$\therefore g'(x) = -x e^x$$

$$g(x) = -(x e^x - \int e^x dx)$$

$$= -x e^x + e^x + C$$

$$\therefore u(x, y) = e^x y - x e^x + e^x + C = 0$$

$$e^x y - x e^x + e^x = C$$

$$y(0) = 4, 4 + 1 = C = 5$$

$$e^x y - x e^x + e^x = 5$$

$$(y - x + 1) = 5/e^x$$

$$\boxed{y = \frac{5}{e^x} + x - 1}$$

$$(6) \frac{dy}{dx} - \frac{4}{x}y = x^6 e^{2x}$$

$$y' - \frac{4}{x}y = x^6 e^{2x}$$

$$-\left(\frac{4}{x}y + x^6 e^{2x}\right)dx + 1 \cdot dy = 0$$

$$P_y = -\left(\frac{4}{x}\right) \quad Q_x = 0$$

$$\frac{1}{Q}(P_y - Q_x) = -\frac{4}{x} = R(x)$$

$$F(x) = e^{\int -\frac{4}{x} dx} = e^{-4 \ln|x|} = x^{-4}$$

$$-\left(\frac{4}{x^5}y + x^2 e^{2x}\right)dx + x^4 dy = 0$$

$$M_y = -\left(\frac{4}{x^5}\right) = N_x = -\frac{4}{x^5}$$

$$U(x, y) = \int x^4 dy = \frac{y}{x^4} + g(x)$$

$$U_x = -\frac{4y}{x^5} + g'(x) = -\frac{4y}{x^5} - x^2 e^{2x}$$

$$g'(x) = -x^2 e^{2x}$$

$$g(x) = -(x^2 e^{2x} - 2 \int x e^{2x} dx)$$

$$= -x^2 e^{2x} + 2x e^{2x} - 2e^{2x} + C$$

$$\therefore U(x, y) = y \cdot x^{-4} - x^2 e^{2x} + 2x e^{2x} - 2e^{2x} + C$$

$$y \cdot x^{-4} - x^2 e^{2x} + 2x e^{2x} - 2e^{2x} = C$$

$$y = x^6 e^{2x} - 2x^5 e^{2x} + 2x^4 e^{2x} + C \cdot x^4$$

$$(8) xy dx + (2x^2 y^2 - 2y) dy = 0$$

$$\frac{xy dx + (2x^2 y^2 - 2y) dy = 0}{P \quad Q}$$

$$P_y = x, \quad Q_x = 4x$$

$$\frac{1}{Q}(Q_x - P_y) = \frac{1}{xy}(4x - x) = \frac{3}{y} = R(y)$$

$$F(y) = e^{\int \frac{3}{y} dy} = e^{3 \ln|y|} = y^3$$

$$y^3 \cdot xy dx + y^3 \cdot (2x^2 y^2 - 2y) dy = 0$$

$$M_y = 4x y^3 = N_x = 4x y^3$$

$$U(x, y) = \frac{1}{2} x^2 y^4 + g(y)$$

$$U_y = 2x^2 y^3 + g'(y) = 2x^2 y^3 + 3y^5 - 2y^3$$

$$g'(y) = 3y^5 - 2y^3$$

$$g(y) = \frac{1}{2} y^6 - 5y^4 + C$$

$$U(x, y) = \frac{1}{2} x^2 y^4 + \frac{1}{2} y^6 - 5y^4 + C$$

$$\frac{1}{2} x^2 y^4 + \frac{1}{2} y^6 - 5y^4 = C$$

$$(7) \frac{dy}{dx} = \frac{x y^2 - \cos x \sin x}{y(1-x^2)}, \quad y(0) = 2$$

$$\frac{(x y^2 - \cos x \sin x) dx + (y(x^2 - 1)) dy = 0}{P \quad Q}$$

$$P_y = 2xy = Q_x = 2xy$$

$$U(x, y) = \frac{1}{2} (x^2 - 1) y^2 + g(x)$$

$$U_x = y^2 x + g'(x) = x y^2 - \cos x \sin x$$

$$g'(x) = -\cos x \sin x$$

$$g(x) = -\int \cos x \sin x dx = \int u du = \frac{1}{2} u^2 + C$$

$$(\cos x = u, -\sin x dx = du)$$

$$\therefore g(x) = \frac{1}{2} \cos^2 x + C$$

$$U(x, y) = \frac{1}{2} (x^2 - 1) y^2 + \frac{1}{2} \cos^2 x + C$$

$$(x^2 - 1) y^2 + \cos^2 x = C$$

$$y(0) = 2, \quad -1 \cdot 4 + 1 = -3 \quad \therefore C = -3$$

$$(x^2 - 1) y^2 + \cos^2 x = -3$$

$$(9) \frac{dy}{dx} = 1 + x + y + xy, \quad y(0) = 0$$

$$\frac{dy}{dx} = (1+x)(1+y)$$

$$\left(\frac{1}{1+y}\right) dy = (1+x) dx$$

$$\int \frac{1}{1+y} dy = \int (1+x) dx$$

$$\ln|1+y| = x + \frac{1}{2} x^2 + C$$

$$y+1 = C e^{x + \frac{1}{2} x^2}$$

$$y = C e^{x + \frac{1}{2} x^2} - 1$$

$$y(0) = 0, \quad 0 = C - 1, \quad C = 1$$

$$y = -1 + e^{x + \frac{1}{2} x^2}$$

2. Given the family of all curves $xy=c$. Find the orthogonal family

$$xy=c$$

$$y + xy' = 0$$

$$y' = -\frac{y}{x}$$

$$\left(-\frac{y}{x}\right) \cdot \left(\frac{x}{y}\right) = -1$$

$$\therefore y' = \frac{x}{y}$$

$$y dy = x dx$$

$$\int y dy = \int x dx$$

$$\frac{1}{2}y^2 = \frac{1}{2}x^2 + C$$

$$\therefore \boxed{x^2 - y^2 = C}$$